theories/Escape.v
@@ -1,73 +1,62 @@
+Require Import CRelationClasses.
 From MetaCoq Require Import PCUICAst.
-Require Import Untyped DeclarativeTyping LogicalRelation Properties Reduction LRInduction.
+Require Import Notations Untyped GenericTyping LogicalRelation Properties Reduction LRInduction.
 Set Universe Polymorphism.
 
-Definition escape {l Γ A} :
-    [Γ ||-< l > A ] ->
-    [Γ |- A].
-Proof.
-  intros [[] lr].
-  cbn in lr.
-  induction lr as [? [] | ? ? [] | ? ? [] ] using LR_rect.
-  - mltt.
-  - mltt.
-  - mltt.
-Qed.
+Section Escapes.
+  Context `{GenericTypingProp}.
 
-Definition escapeEq {l Γ A B} (lr : [Γ ||-< l > A]) :
-    [ Γ ||-< l > A ≅ B | lr ] ->
-    [Γ |- A ≅ B].
-Proof.
-  destruct lr as [[] lr].
-  cbn in *.
-  induction lr as [ ? [] | ? ? [] | ? ? [] IHdom IHcod] using LR_rect.
-  + intros [->].
-    mltt.
-  + intros [].
-    do 2 eapply TypeTrans.
-    all: mltt.
-  + intros [] ; cbn in *.
-    do 2 eapply TypeTrans.
-    all: mltt.
-Qed.
+  Definition escape {l Γ A} :
+      [Γ ||-< l > A ] ->
+      [Γ |- A].
+  Proof.
+    intros [[] lr].
+    cbn in lr.
+    red in lr.
+    induction lr as [? [] | ? ? [] | ? ? [] ].
+    all: gen_typing.
+  Qed.
 
-Definition escapeTerm {l Γ t A} (lr : [Γ ||-< l > A ]) :
-  [Γ ||-< l > t : A | lr ] ->
-  [Γ |- t : A].
-Proof.
-  destruct lr as [[] lr].
-  cbn in *.
-  induction lr as [ ? [] | ? ? [] | ? ? [] IHdom IHcod] using LR_rect.
-  all: intros [] ; cbn in *.
-  all: mltt.
-Qed.
+  Definition escapeEq {l Γ A B} (lr : [Γ ||-< l > A]) :
+      [ Γ ||-< l > A ≅ B | lr ] ->
+      [Γ |- A ≅ B].
+  Proof.
+    destruct lr as [[] lr].
+    cbn in *.
+    induction lr as [ ? [] | ? ? [] | ? ? [] IHdom IHcod].
+    + intros [->].
+      gen_typing.
+    + intros [].
+      cbn in *.
+      gen_typing.
+    + intros [].
+      cbn in *.
+      gen_typing.
+  Qed.
 
-Definition escapeEqTerm {l Γ t u A} (lr : [Γ ||-< l > A ]) :
-  [Γ ||-< l > t ≅ u : A | lr ] ->
-  [Γ |- t ≅ u: A].
-Proof.
-  destruct lr as [[] lr].
-  cbn in *.
-  induction lr as [ ? [] | ? ? [] | ? ? [] IHdom IHcod] using LR_rect.
-  - intros [[termL] [termR]] ; cbn in *.
-    eapply (TermTrans (t' := termL)).
-    1: mltt.
-    eapply (TermTrans (t' := termR)).
-    1: mltt.
-    eapply TermConv.
-    all: mltt.
-  - intros [] ; cbn in *.
-    eapply (TermTrans (t' := termL)).
-    1: mltt.
-    eapply (TermTrans (t' := termR)).
-    1: mltt.
-    eapply TermConv.
-    all: mltt.
-  - intros [[termL] [termR]] ; cbn in *.
-    eapply (TermTrans (t' := termL)).
-    1: mltt.
-    eapply (TermTrans (t' := termR)).
-    1: mltt.
-    eapply TermConv.
-    all: mltt.
-Qed.
+  Definition escapeTerm {l Γ t A} (lr : [Γ ||-< l > A ]) :
+    [Γ ||-< l > t : A | lr ] ->
+    [Γ |- t : A].
+  Proof.
+    destruct lr as [[] lr].
+    cbn in *.
+    induction lr as [ ? [] | ? ? [] | ? ? [] IHdom IHcod].
+    all: intros [] ; cbn in *.
+    all: gen_typing.
+  Qed.
+
+  Definition escapeEqTerm {l Γ t u A} (lr : [Γ ||-< l > A ]) :
+    [Γ ||-< l > t ≅ u : A | lr ] ->
+    [Γ |- t ≅ u : A].
+  Proof.
+    destruct lr as [[] lr].
+    cbn in *.
+    induction lr as [ ? [] | ? ? [] | ? ? [] IHdom IHcod].
+    - intros [[termL] [termR]] ; cbn in *.
+      gen_typing.
+    - intros [] ; cbn in *.
+      eapply convtm_exp.
+      all: gen_typing.
+    - intros [[termL] [termR]] ; cbn in *.
+      gen_typing.
+  Qed.
