theories/LRInduction.v
@@ -1,114 +1,122 @@
 From MetaCoq.PCUIC Require Import PCUICAst PCUICRenameConv PCUICInstConv PCUICSigmaCalculus.
-From LogRel Require Import Notations Untyped Weakening DeclarativeTyping LogicalRelation.
+From LogRel Require Import Notations Untyped Weakening GenericTyping LogicalRelation.
 
-#[universes(polymorphic)]Fixpoint LR_embedding {l l'} (l_ : l << l')
-  {Γ A rEq rTe rTeEq} (lr : LRl l Γ A rEq rTe rTeEq) {struct lr} : (LRl l' Γ A rEq rTe rTeEq) :=
-  match lr with
-   | LRU Γ H =>
-      match
-        (match l_ with Oi => fun H' => elim H'.(URedTy.lt) end H)
-      with end
-   | LRne _ _ neA => LRne _ neA
-   | LRPi _ _ ΠA ΠAad => LRPi _ ΠA
-      {|
-        PiRedTy.domAd :=
-          fun (Δ : context) (ρ : Δ ≤ _) (h : [  |- Δ]) => LR_embedding l_ (ΠAad.(PiRedTy.domAd) ρ h) ;
-        PiRedTy.codAd :=
-          fun (Δ : context) (a : term) (ρ : Δ ≤ _) (h : [  |- Δ])
-            (ha : [PiRedTy.domRed ΠA ρ h | Δ ||- a : _]) =>
-          LR_embedding l_ (ΠAad.(PiRedTy.codAd) ρ h ha)
-      |}
-  end.
+Section Inductions.
+  Context `{ta : tag}
+    `{!WfContext ta} `{!WfType ta} `{!Typing ta}
+    `{!ConvType ta} `{!ConvTerm ta} `{!ConvNeu ta}
+    `{!OneRedType ta} `{!OneRedTerm ta}.
 
-#[universes(polymorphic)]Theorem LR_rect
-  (l : TypeLevel)
-  (rec : forall l', l' << l -> LogRelKit)
-  (P : forall {c t rEq rTe rTeEq},
-    LR rec c t rEq rTe rTeEq  -> Type) :
+  #[universes(polymorphic)]Fixpoint LR_embedding {l l'} (l_ : l << l')
+    {Γ A rEq rTe rTeEq} (lr : LRl l Γ A rEq rTe rTeEq) {struct lr} : (LRl l' Γ A rEq rTe rTeEq) :=
+    match lr with
+    | LRU Γ H =>
+        match
+          (match l_ with Oi => fun H' => elim H'.(URedTy.lt) end H)
+        with end
+    | LRne _ _ neA => LRne _ neA
+    | LRPi _ _ ΠA ΠAad => LRPi _ ΠA
+        {|
+          PiRedTy.domAd :=
+            fun (Δ : context) (ρ : Δ ≤ _) (h : [  |- Δ]) => LR_embedding l_ (ΠAad.(PiRedTy.domAd) ρ h) ;
+          PiRedTy.codAd :=
+            fun (Δ : context) (a : term) (ρ : Δ ≤ _) (h : [  |- Δ])
+              (ha : [PiRedTy.domRed ΠA ρ h | Δ ||- a : _]) =>
+            LR_embedding l_ (ΠAad.(PiRedTy.codAd) ρ h ha)
+        |}
+    end.
 
-  (forall (Γ : context) (h : [Γ ||-U l]),
-    P (LRU rec h)) ->
+  #[universes(polymorphic)]Theorem LR_rect
+    (l : TypeLevel)
+    (rec : forall l', l' << l -> LogRelKit)
+    (P : forall {c t rEq rTe rTeEq},
+      LR rec c t rEq rTe rTeEq  -> Type) :
 
-  (forall (Γ : context) (A : term) (neA : [Γ ||-ne A]),
-    P (LRne rec neA)) ->
+    (forall (Γ : context) (h : [Γ ||-U l]),
+      P (LRU rec h)) ->
 
-  (forall (Γ : context) (A : term) (ΠA : [ Γ ||-Πd A ]) (HAad : PiRedTyAdequate (LR rec) ΠA),
-  (forall {Δ} (ρ : Δ ≤ Γ) (h : [ |- Δ]),
-    P (HAad.(PiRedTy.domAd) ρ h)) ->
-  (forall {Δ a} (ρ : Δ ≤ Γ) (h : [ |- Δ ]) 
-    (ha : [ ΠA.(PiRedTy.domRed) ρ h | Δ ||- a : ΠA.(PiRedTy.dom).[ren ρ] ]),
-  P (HAad.(PiRedTy.codAd) ρ h ha)) ->
-  P (LRPi rec ΠA HAad)) ->
+    (forall (Γ : context) (A : term) (neA : [Γ ||-ne A]),
+      P (LRne rec neA)) ->
 
-  forall (Γ : context) (t : term) (rEq rTe : term -> Type)
-    (rTeEq  : term -> term -> Type) (lr : LR rec Γ t rEq rTe rTeEq),
-    P lr.
-Proof.
-  cbn.
-  intros HU Hne HPi.
-  fix HRec 6.
-  destruct lr.
-  - eapply HU.
-  - eapply Hne.
-  - eapply HPi.
-    all: intros ; eapply HRec.
-Qed.
+    (forall (Γ : context) (A : term) (ΠA : [ Γ ||-Πd A ]) (HAad : PiRedTyAdequate (LR rec) ΠA),
+    (forall {Δ} (ρ : Δ ≤ Γ) (h : [ |- Δ]),
+      P (HAad.(PiRedTy.domAd) ρ h)) ->
+    (forall {Δ a} (ρ : Δ ≤ Γ) (h : [ |- Δ ]) 
+      (ha : [ ΠA.(PiRedTy.domRed) ρ h | Δ ||- a : ΠA.(PiRedTy.dom).[ren ρ] ]),
+    P (HAad.(PiRedTy.codAd) ρ h ha)) ->
+    P (LRPi rec ΠA HAad)) ->
 
-Theorem LR_rect_LogRelRec
-  (P : forall {l Γ t rEq rTe rTeEq},
-  LRl l Γ t rEq rTe rTeEq  -> Type) :
+    forall (Γ : context) (t : term) (rEq rTe : term -> Type)
+      (rTeEq  : term -> term -> Type) (lr : LR rec Γ t rEq rTe rTeEq),
+      P lr.
+  Proof.
+    cbn.
+    intros HU Hne HPi.
+    fix HRec 6.
+    destruct lr.
+    - eapply HU.
+    - eapply Hne.
+    - eapply HPi.
+      all: intros ; eapply HRec.
+  Qed.
 
-  (forall (Γ : context) (h : [Γ ||-U one]),
-    P (LRU (rec1) h)) ->
+  Theorem LR_rect_LogRelRec
+    (P : forall {l Γ t rEq rTe rTeEq},
+    LRl l Γ t rEq rTe rTeEq  -> Type) :
 
-  (forall (l : TypeLevel) (Γ : context) (A : term) (neA : [Γ ||-ne A]),
-    P (LRne (LogRelRec l) neA)) ->
+    (forall (Γ : context) (h : [Γ ||-U one]),
+      P (LRU (rec1) h)) ->
 
-  (forall (l : TypeLevel) (Γ : context) (A : term) (ΠA : [ Γ ||-Πd A ])
-    (HAad : PiRedTyAdequate (LRl l) ΠA),
-  (forall {Δ} (ρ : Δ ≤ Γ) (h : [ |- Δ]),
-    P (HAad.(PiRedTy.domAd) ρ h)) ->
-  (forall {Δ a} (ρ : Δ ≤ Γ) (h : [ |- Δ ]) 
-    (ha : [ ΠA.(PiRedTy.domRed) ρ h | Δ ||- a : ΠA.(PiRedTy.dom).[ren ρ] ]),
-  P (HAad.(PiRedTy.codAd) ρ h ha)) ->
-  P (LRPi (LogRelRec l) ΠA HAad)) ->
+    (forall (l : TypeLevel) (Γ : context) (A : term) (neA : [Γ ||-ne A]),
+      P (LRne (LogRelRec l) neA)) ->
 
-  forall (l : TypeLevel) (Γ : context) (t : term) (rEq rTe : term -> Type)
-    (rTeEq  : term -> term -> Type) (lr : LR (LogRelRec l) Γ t rEq rTe rTeEq),
-    P lr.
-Proof.
-  intros.
-  apply LR_rect.
-  - intros.
-    destruct l.
-    2: auto.
-    destruct h as [? lt].
-    inversion lt.
-  - auto.
-  - auto.
-Qed.
+    (forall (l : TypeLevel) (Γ : context) (A : term) (ΠA : [ Γ ||-Πd A ])
+      (HAad : PiRedTyAdequate (LRl l) ΠA),
+    (forall {Δ} (ρ : Δ ≤ Γ) (h : [ |- Δ]),
+      P (HAad.(PiRedTy.domAd) ρ h)) ->
+    (forall {Δ a} (ρ : Δ ≤ Γ) (h : [ |- Δ ]) 
+      (ha : [ ΠA.(PiRedTy.domRed) ρ h | Δ ||- a : ΠA.(PiRedTy.dom).[ren ρ] ]),
+    P (HAad.(PiRedTy.codAd) ρ h ha)) ->
+    P (LRPi (LogRelRec l) ΠA HAad)) ->
 
-Theorem LR_rect_TyUr
-  (P : forall {l Γ A}, [Γ ||-< l > A] -> Type) :
+    forall (l : TypeLevel) (Γ : context) (t : term) (rEq rTe : term -> Type)
+      (rTeEq  : term -> term -> Type) (lr : LR (LogRelRec l) Γ t rEq rTe rTeEq),
+      P lr.
+  Proof.
+    intros.
+    apply LR_rect.
+    - intros.
+      destruct l.
+      2: auto.
+      destruct h as [? lt].
+      inversion lt.
+    - auto.
+    - auto.
+  Qed.
 
-  (forall (Γ : context) (h : [Γ ||-U one]),
-    P (LRU_ h)) ->
+  Theorem LR_rect_TyUr
+    (P : forall {l Γ A}, [Γ ||-< l > A] -> Type) :
 
-  (forall (l : TypeLevel) (Γ : context) (A : term) (neA : [Γ ||-ne A]),
-    P (LRne_ l neA)) ->
+    (forall (Γ : context) (h : [Γ ||-U one]),
+      P (LRU_ h)) ->
 
-  (forall (l : TypeLevel) (Γ : context) (A : term) (ΠA : [ Γ ||-Πd A ]) (HAad : PiRedTyAdequate (LRl l) ΠA),
-  (forall {Δ} (ρ : Δ ≤ Γ) (h : [ |- Δ]),
-    P (LRbuild (HAad.(PiRedTy.domAd) ρ h))) ->
-  (forall {Δ a} (ρ : Δ ≤ Γ) (h : [ |- Δ ]) 
-    (ha : [ ΠA.(PiRedTy.domRed) ρ h | Δ ||- a : ΠA.(PiRedTy.dom).[ren ρ] ]),
-  P (LRbuild (HAad.(PiRedTy.codAd) ρ h ha))) ->
-  P (LRPi_ l ΠA HAad)) ->
+    (forall (l : TypeLevel) (Γ : context) (A : term) (neA : [Γ ||-ne A]),
+      P (LRne_ l neA)) ->
 
-  forall (l : TypeLevel) (Γ : context) (A : term) (lr : [Γ ||-< l > A]),
-    P lr.
-Proof.
-  intros HU Hne HPi l Γ A lr.
-  apply (LR_rect_LogRelRec (fun l Γ A _ _ _ lr => P l Γ A (LRbuild lr))).
-  all: auto.
-Qed.
+    (forall (l : TypeLevel) (Γ : context) (A : term) (ΠA : [ Γ ||-Πd A ]) (HAad : PiRedTyAdequate (LRl l) ΠA),
+    (forall {Δ} (ρ : Δ ≤ Γ) (h : [ |- Δ]),
+      P (LRbuild (HAad.(PiRedTy.domAd) ρ h))) ->
+    (forall {Δ a} (ρ : Δ ≤ Γ) (h : [ |- Δ ]) 
+      (ha : [ ΠA.(PiRedTy.domRed) ρ h | Δ ||- a : ΠA.(PiRedTy.dom).[ren ρ] ]),
+    P (LRbuild (HAad.(PiRedTy.codAd) ρ h ha))) ->
+    P (LRPi_ l ΠA HAad)) ->
+
+    forall (l : TypeLevel) (Γ : context) (A : term) (lr : [Γ ||-< l > A]),
+      P lr.
+  Proof.
+    intros HU Hne HPi l Γ A lr.
+    apply (LR_rect_LogRelRec (fun l Γ A _ _ _ lr => P l Γ A (LRbuild lr))).
+    all: auto.
+  Qed.
+
+End Inductions.
